verif/verif_movetonext.v
@@ -20,14 +20,171 @@ Require Import verif_movetofirst.
 Lemma body_lastpointer: semax_body Vprog Gprog f_lastpointer lastpointer_spec.
 Proof.
   start_function.
+  destruct n as [ptr0 le isLeaf First Last pn].
+  pose (n:=btnode val ptr0 le isLeaf First Last pn).
+  rewrite unfold_btnode_rep. Intros.
+  forward.                      (* t'1=node->isLeaf *)
+  { entailer!. destruct isLeaf; simpl; auto. }
+  forward_if.
+  - forward.                    (* t'3=node->numKeys *)
+    forward.                    (* return *)
+    entailer!.
+    destruct isLeaf.
+    + unfold rep_index. reflexivity.
+    + simpl in H0. inv H0.
+  - forward.                    (* t'2=node->numKeys *)
+    forward.                    (* return *)
+    { entailer!. unfold node_wf in H.
+      simpl in H. clear -H. admit. (* OK *) }
+    entailer!.
+    destruct isLeaf.
+    + simpl in H0. inv H0.
+    + destruct (numKeys_le le).
+      * unfold rep_index. simpl. reflexivity.
+      * assert (Z.of_nat (S n0) -1 = Z.of_nat n0).
+        { admit. }              (* OK *)
+        rewrite H6. unfold rep_index. reflexivity.  
 Admitted.
 
 Lemma body_moveToNext: semax_body Vprog Gprog f_moveToNext moveToNext_spec.
 Proof.
   start_function.
+  destruct r as [[[root numRec] depth] prel].
+  pose (r:=(root,numRec,depth,prel)). fold r.
+  destruct c as [|[n i] c'].
+  inv H0. pose (c:=(n,i)::c'). fold c.
+  unfold cursor_rep. Intros anc_end. Intros idx_end. unfold r.
+  forward.                      (* t'17=cursor->relation *)
+  unfold relation_rep. Intros.
+  forward.                      (* t'18=t'17->numRecords *)
+  forward_if.
+  {  forward.                   (* return *)
+     assert (numRec = O) by admit. (* OK by H1 *)
+     entailer!.
+     unfold moveToNext. simpl. fold c. unfold cursor_rep. Exists anc_end. Exists idx_end. cancel. }
+  forward.                      (* skip *)
+  forward_call(r,c,pc).         (* t'1=isValid(cursor) *)
+  { unfold relation_rep, cursor_rep. unfold r. Exists anc_end. Exists idx_end. cancel.
+    change_compspecs CompSpecs. cancel. }
+  forward_if.
+  { forward.                    (* return *)
+    assert (isValid c r = false) by admit. (* OK by H2 *)
+    assert (moveToNext c r = c).
+    { unfold moveToNext. destruct (get_numrec r). auto. rewrite H8. auto. }
+    fold c. fold r. rewrite H9.
+    entailer!.  }
+  forward.                      (* skip *)
+  assert (isValid c r = true).
+  { destruct (isValid c r). auto. inv H2. } rewrite H3.
+  forward_loop
+    (EX i:Z, PROP()
+             LOCAL (temp _t'1 (Val.of_bool true); temp _t'18 (Vint (Int.repr (Z.of_nat numRec))); temp _t'17 prel; temp _cursor pc)
+             SEP (relation_rep r; cursor_rep (sublist 0 (Zlength c - i) c) r pc))
+    break:(PROP()
+           LOCAL (temp _t'1 (Val.of_bool true); temp _t'18 (Vint (Int.repr (Z.of_nat numRec))); temp _t'17 prel; temp _cursor pc)
+           SEP (relation_rep r; cursor_rep (up_at_last c) r pc)).
+  - Exists 0. entailer!. rewrite sublist_same. cancel. auto. omega.
+  - Intros i0.
+    pose (subc:=sublist 0 (Zlength c - i0) c). fold subc.
+    unfold cursor_rep.
+    Intros anc_end0. Intros idx_end0. unfold r.
+    forward.                    (* t'16 = cursor->level *)
+    gather_SEP 1 2. replace_SEP 0 (cursor_rep subc r pc).
+    { entailer!. unfold cursor_rep. Exists anc_end0. Exists idx_end0. unfold r. cancel. }
+    forward_if (PROP ( )
+     LOCAL (temp _t'16 (Vint (Int.repr (Zlength subc - 1))); temp _t'1 (Val.of_bool true);
+            temp _t'18 (Vint (Int.repr (Z.of_nat numRec))); temp _t'17 prel; temp _cursor pc;
+            temp _t'2 (Val.of_bool (andb (Z.gtb (Zlength subc - 1) 0) (index_eqb i (lastpointer n))))) 
+     SEP (cursor_rep subc r pc; relation_rep (root, numRec, depth, prel))).
+    + forward_call(r,subc,pc).     (* t'3=entryInde(cursor) *)
+      { fold r. cancel. }
+      { admit.                  (* todo: cursor_wf preserved *) }
+      forward_call(r,subc,pc).
+      { admit.                  (* todo: cursor_wf preserved *) }
+      forward_call(currNode subc r). (* 't'5=lastpointer t'4 *)
+      { admit. }
+      { admit.                  (* todo: node_wf preserved *) }
+      forward.                  (* t'2= (t'3==t'5) *)
+      entailer!.
+      admit.
+      admit.
+    + forward.                  (* t'2=0 *)
+      entailer!.
+      admit.
+    + forward_if.
+      * forward.                (* skip *)
+        unfold cursor_rep. unfold r. Intros anc_end1. Intros idx_end1.
+        forward.                (* t'15=cursor->level *)
+        forward.                (* cursor->level = t'15-1 *)
+        { admit. }
+        Exists (i0+1). entailer!. unfold cursor_rep. unfold r.
+        Exists ((getval (currNode subc r))::anc_end1).
+        Exists ((rep_index(entryIndex subc))::idx_end1).
+        cancel.
+        admit.                  (* should be ok *)
+      * forward.                (* break *)
+        entailer!.
+        admit. (* TODO: prove that when the loop stops, we have up_at_last *)
+  - unfold cursor_rep. Intros anc_end0. Intros idx_end0. unfold r.
+    forward.                    (* t'12=cursor->level *)
+    forward.                    (* t'13=cursor->level *)
+    forward.                    (* t'14=cursor->ancidx[t'13] *)
+    { admit.                    (* cursor in range *) }
+    { admit. }
+    forward.                    (* cursor->ancestors[t'12] = t'14 +1 *)
+    { admit. }
+    { admit. }
+    gather_SEP 1 2. pose(cincr := next_cursor (up_at_last c)).
+    replace_SEP 0 (cursor_rep cincr r pc).
+    { unfold cursor_rep. entailer!.
+    Exists anc_end0. Exists idx_end0. cancel. admit. }
+    forward_call(r,cincr,pc).       (* t'6=currNode(cursor) *)
+    { fold r. cancel. }
+    { admit. }
+    destruct (currNode cincr r).
+    simpl. Intros.
+    (* here I need a representation for the current node of cincr *)
+    admit.
 Admitted.
 
 Lemma body_RL_MoveToNext: semax_body Vprog Gprog f_RL_MoveToNext RL_MoveToNext_spec.
 Proof.
   start_function.
+  destruct r as [[[root numRec] depth] prel].
+  pose (r:=(root,numRec,depth,prel)). fold r.
+  destruct c as [|[n i] c'].
+  inv H0. pose (c:=(n,i)::c'). fold c.
+  forward_call(r,c,pc).         (* t'1=entryIndex(cursor) *)
+  forward_call(r,c,pc).         (* t'2=currNode(cursor) *)
+  unfold c. simpl.
+  destruct n as [ptr0 le isLeaf First Last pn].
+  pose (n:=btnode val ptr0 le isLeaf First Last pn). simpl.
+  assert (subnode n root) by admit. (* I need a cursor correctness property here *)
+  unfold relation_rep. rewrite subnode_rep with (n:=n) by auto.
+  rewrite unfold_btnode_rep at 1. unfold n. Intros.
+  forward.                      (* t'3=t'2->numKeys *)
+  simpl.
+  gather_SEP 2 3 4 5. replace_SEP 0 (btnode_rep n).
+  { entailer!. } gather_SEP 0 3. replace_SEP 0 (btnode_rep root).
+  { entailer!. apply wand_frame_elim. } gather_SEP 0 1 2. replace_SEP 0 (relation_rep r).
+  { entailer!. } fold c.
+  forward_if(PROP ( )
+     LOCAL (temp _t'3 (Vint (Int.repr (Z.of_nat (numKeys_le le)))); temp _t'2 pn;
+     temp _t'1 (rep_index i); temp _cursor pc)
+     SEP (relation_rep r; match (index_eqb i (ip (numKeys n))) with true => cursor_rep (moveToNext c r) r pc | false => cursor_rep c r pc end)).
+  - forward_call(c,pc,r).       (* moveToNext(cursor) *)
+    entailer!.
+    assert (i = ip (numKeys_le le)) by admit. (* OK by H2 *)
+    rewrite H10. simpl. admit.                          (* OK *)
+  - forward.                                            (* skip *)
+    assert (i <> ip (numKeys n)) by admit. (* OK by H2 *)
+    entailer!. admit.                                   (* OK *)
+  - forward_call(c,pc,r).                               (* moveToNext(cursor) *)
+    + admit.                                            (* false *)
+    + forward.                                          (* return *)
+      entailer!.
+      * admit.                  (* todo: cursor_wf & cursor_correct preservation *)
+      * admit.                  (* false *)
 Admitted.
+(* Why is there no match in the POSTCONDITION? *)
+        
